Well-formedness of constructor now only uses a type environment

src/Language/PlutusIR/Semantics/Dynamic/Smallstep.v
@@ -1,6 +1,7 @@
 Require Import PlutusCert.Language.PlutusIR.
 Import NamedTerm.
 Require Export PlutusCert.Language.PlutusIR.Semantics.Dynamic.BuiltinMeanings.
+Require Export PlutusCert.Language.PlutusIR.Semantics.Dynamic.AnnotationSubstitution.
 Require Export PlutusCert.Language.PlutusIR.Semantics.Dynamic.Substitution.
 Require Export PlutusCert.Language.PlutusIR.Semantics.Dynamic.Values.
 
@@ -9,42 +10,58 @@ Require Export PlutusCert.Language.PlutusIR.Semantics.Dynamic.Values.
 Create HintDb smallstep_db.
 
 Reserved Notation "t '-->' t'" (at level 40).
+
+
 Inductive step : Term -> Term -> Prop :=
   (* Let-bindings *)
-  | ST_Let : forall bs t t',
-      step_bindings_nonrec (Let NonRec bs t) t' ->
-      step (Let NonRec bs t) t'
-  (* TyAbs *)
-  | ST_TyAbs : forall X K t t',
-      t --> t' ->
-      TyAbs X K t --> TyAbs X K t'
-
+  | ST_Let_NilB : forall recty t,
+      Let recty nil t --> t
+  | ST_LetNonRec_ConsB1 : forall s x T tb bs t tb',
+      tb --> tb' ->
+      Let NonRec ((TermBind s (VarDecl x T) tb) :: bs) t -->
+        Let NonRec ((TermBind s (VarDecl x T) tb') :: bs) t
+  | ST_LetNonRec_ConsB2 :  forall s x T vb bs t bs' t',
+      value vb ->
+      substitute x vb (Let NonRec bs t) (Let NonRec bs' t') ->
+      Let NonRec ((TermBind s (VarDecl x T) vb) :: bs) t --> Let NonRec bs' t'
   (* Apply *)
   | ST_Apply1 : forall t1 t1' t2,
       t1 --> t1' ->
       Apply t1 t2 --> Apply t1' t2
-  | ST_Apply2 : forall v1 t2 t2',
-      value v1 ->
+  | ST_Apply2 : forall x T t0 t2 t2',
       t2 --> t2' ->
-      Apply v1 t2 --> Apply v1 t2'
+      Apply (LamAbs x T t0) t2 --> Apply (LamAbs x T t0) t2'
   | ST_ApplyLamAbs : forall x T t0 v2 t0',
       value v2 ->
       substitute x v2 t0 t0' ->
       Apply (LamAbs x T t0) v2 --> t0'
   (* Builtins *)
-  | ST_ApplyBuiltin2 : forall v1 v2 v0,
+  | ST_Apply3 : forall v1 t2 t2',
+      value_builtin v1 ->
+      t2 --> t2' ->
+      Apply v1 t2 --> Apply v1 t2' 
+  | ST_ApplyBuiltin : forall v1 v2 v0,
       value_builtin v1 ->
       value v2 ->
       ~(value_builtin (Apply v1 v2)) ->
       compute_defaultfun (Apply v1 v2) = Datatypes.Some v0 ->
       Apply v1 v2 --> v0
+  (* If-Then-Else *)
+  | ST_ApplyIf : forall cond cond' T then_branch else_branch,
+      cond --> cond' ->
+      Apply (Apply (Apply (TyInst (Builtin IfThenElse) T) cond) then_branch) else_branch --> Apply (Apply (Apply (TyInst (Builtin IfThenElse) T) cond') then_branch) else_branch
+  | ST_ApplyIfTrue : forall T then_branch else_branch,
+      Apply (Apply (Apply (TyInst (Builtin IfThenElse) T) (Constant (Some (ValueOf DefaultUniBool true)))) then_branch) else_branch --> then_branch
+  | ST_ApplyIfFalse : forall T then_branch else_branch, 
+      Apply (Apply (Apply (TyInst (Builtin IfThenElse) T) (Constant (Some (ValueOf DefaultUniBool true)))) then_branch) else_branch --> else_branch
 
   (* TyInst *)
   | ST_TyInst1 : forall t1 t1' T,
       t1 --> t1' ->
       TyInst t1 T --> TyInst t1' T
-  | ST_TyInstTyAbs : forall X K v0 T,
-      TyInst (TyAbs X K v0) T --> v0 
+  | ST_TyInstTyAbs : forall X K v0 T v0',
+      substituteA X T v0 v0' ->
+      TyInst (TyAbs X K v0) T --> v0' 
 
   (* Wrap and unwrap *)
   | ST_IWrap : forall F T t0 t0',
@@ -57,27 +74,32 @@ Inductive step : Term -> Term -> Prop :=
       Unwrap (IWrap F T v0) --> v0
 
   (* Errors *)
-
-with step_bindings_nonrec : Term -> Term -> Prop :=
-  | ST_NilB_NonRec1 : forall t t',
-      t --> t' ->
-      step_bindings_nonrec (Let NonRec nil t) (Let NonRec nil t')
-  | ST_NilB_NonRec2 : forall v,
-      value v ->
-      step_bindings_nonrec (Let NonRec nil v) v
-  | ST_ConsB_NonRec1 : forall s x T tb bs t tb',
-      tb --> tb' ->
-      step_bindings_nonrec (Let NonRec ((TermBind s (VarDecl x T) tb) :: bs) t) (Let NonRec ((TermBind s (VarDecl x T) tb') :: bs) t)
-  | ST_ConsB_NonRec2 : forall s x T vb bs t bs' t',
-      value vb ->
-      substitute_bindings_nonrec x vb bs bs' ->
-      substitute x vb t t' ->
-      step_bindings_nonrec (Let NonRec ((TermBind s (VarDecl x T) vb) :: bs) t) (Let NonRec bs' t')
+  | ST_Apply1_Error : forall T_err t1 t2,
+      t1 --> Error T_err ->
+      Apply t1 t2 --> Error T_err
+  | ST_Apply2_Error : forall T_err x T t0 t2,
+      t2 --> Error T_err ->
+      Apply (LamAbs x T t0) t2 --> Error T_err
+  | ST_Apply3_Error : forall T_err v1 t2,
+      value_builtin v1 ->
+      t2 --> Error T_err ->
+      Apply v1 t2 --> Error T_err
+  | ST_ApplyIf_Error : forall cond T T_err then_branch else_branch,
+      cond --> Error T_err ->
+      Apply (Apply (Apply (TyInst (Builtin IfThenElse) T) cond) then_branch) else_branch --> Error T_err
+  | ST_TyInst1_Error : forall t1 T T_err,
+      t1 --> Error T_err ->
+      TyInst t1 T --> Error T_err
+  | ST_IWrap_Error : forall F T t0 T_err,
+      t0 --> Error T_err ->
+      IWrap F T t0 --> Error T_err
+  | ST_Unwrap_Error : forall t0 T_err,
+      t0 --> Error T_err ->
+      Unwrap t0 --> Error T_err
 
 where "t '-->' t'" := (step t t').
 
 #[export] Hint Constructors step : smallstep_db.
-#[export] Hint Constructors step_bindings_nonrec : smallstep_db.
 
 (* Multistep reduction *)
 
@@ -90,8 +112,6 @@ Inductive multi {X : Type} (R : X -> X -> Prop) (x : X) : X -> Prop :=
 Notation multistep := (multi step).
 
 Notation "t1 '-->*' t2" := (multistep t1 t2) (at level 40).
-
-Notation multistepBNR := (multi step_bindings_nonrec).
 
 #[export] Hint Constructors multi : smallstep_db.
 
