src/Language/PlutusIR/Semantics/Dynamic/Equivalence.v
@@ -1,9 +1,12 @@
 Require Import PlutusCert.Language.PlutusIR.
 Import NamedTerm.
 Require Import PlutusCert.Language.PlutusIR.Semantics.Dynamic.Bigstep.
+Require Import PlutusCert.Language.PlutusIR.Semantics.Dynamic.Bigstep.Deterministic.
 Require Import PlutusCert.Language.PlutusIR.Semantics.Dynamic.Bigstep.EvalToValue.
+Require Import PlutusCert.Language.PlutusIR.Semantics.Dynamic.Bigstep.EvalValue.
 Require Import PlutusCert.Language.PlutusIR.Semantics.Dynamic.Smallstep.
 
+(*
 Lemma multistep_congr_Let : forall bs t t',
     multistepBNR (Let NonRec bs t) t' ->
     Let NonRec bs t -->* t'.
@@ -238,5 +241,442 @@ Proof.
       assumption.
     }
     apply multi_refl.
+Qed.*)
+
+Lemma compute_defaultfun__LamAbs : forall t x T t0,
+  compute_defaultfun t <> Datatypes.Some (LamAbs x T t0).
+Proof.
+  intros.
+  intros Hcon.
+  destruct t.
+  all: inversion Hcon.
+  destruct t1; try discriminate.
+  - destruct t1_1; try discriminate.
+    + destruct t1_1_1; try discriminate.
+      destruct d; try discriminate.
+      destruct t1_1_2; try discriminate.
+      destruct s; try discriminate.
+      destruct u; try discriminate.
+      destruct v; try discriminate.
+      destruct t1_2; try discriminate.
+      destruct s; try discriminate.
+      destruct u0; try discriminate.
+      destruct v; try discriminate.
+      destruct t2; try discriminate.
+      destruct s; try discriminate.
+      destruct u1; try discriminate.
+      destruct v; try discriminate.
+    + destruct d; try discriminate.
+      all: try solve [
+        destruct t1_2; try discriminate;
+        destruct s; try discriminate;
+        destruct u; try discriminate;
+        destruct v; try discriminate;
+        destruct t2; try discriminate;
+        destruct s; try discriminate;
+        destruct u0; try discriminate;
+        destruct v; try discriminate
+      ].
+  - destruct d; try discriminate.
+    all: try solve [
+      destruct t2; try discriminate;
+      destruct s; try discriminate;
+      destruct u; try discriminate;
+      destruct v; try discriminate
+    ].
 Qed.
 
+Lemma compute_defaultfun__IfThenElse0 : forall t T0,
+  compute_defaultfun t <> Datatypes.Some (TyInst (Builtin IfThenElse) T0).
+Proof.
+  intros.
+  intros Hcon.
+  destruct t.
+  all: inversion Hcon.
+  destruct t1; try discriminate.
+  - destruct t1_1; try discriminate.
+    + destruct t1_1_1; try discriminate.
+      destruct d; try discriminate.
+      destruct t1_1_2; try discriminate.
+      destruct s; try discriminate.
+      destruct u; try discriminate.
+      destruct v; try discriminate.
+      destruct t1_2; try discriminate.
+      destruct s; try discriminate.
+      destruct u0; try discriminate.
+      destruct v; try discriminate.
+      destruct t2; try discriminate.
+      destruct s; try discriminate.
+      destruct u1; try discriminate.
+      destruct v; try discriminate.
+    + destruct d; try discriminate.
+      all: try solve [
+        destruct t1_2; try discriminate;
+        destruct s; try discriminate;
+        destruct u; try discriminate;
+        destruct v; try discriminate;
+        destruct t2; try discriminate;
+        destruct s; try discriminate;
+        destruct u0; try discriminate;
+        destruct v; try discriminate
+      ].
+  - destruct d; try discriminate.
+    all: try solve [
+      destruct t2; try discriminate;
+      destruct s; try discriminate;
+      destruct u; try discriminate;
+      destruct v; try discriminate
+    ].
+Qed.
+
+Lemma compute_defaultfun__IfThenElse1 : forall t T0 cond,
+  compute_defaultfun t <> Datatypes.Some (Apply (TyInst (Builtin IfThenElse) T0) cond).
+Proof.
+  intros.
+  intros Hcon.
+  destruct t.
+  all: inversion Hcon.
+  destruct t1; try discriminate.
+  - destruct t1_1; try discriminate.
+    + destruct t1_1_1; try discriminate.
+      destruct d; try discriminate.
+      destruct t1_1_2; try discriminate.
+      destruct s; try discriminate.
+      destruct u; try discriminate.
+      destruct v; try discriminate.
+      destruct t1_2; try discriminate.
+      destruct s; try discriminate.
+      destruct u0; try discriminate.
+      destruct v; try discriminate.
+      destruct t2; try discriminate.
+      destruct s; try discriminate.
+      destruct u1; try discriminate.
+      destruct v; try discriminate.
+    + destruct d; try discriminate.
+      all: try solve [
+        destruct t1_2; try discriminate;
+        destruct s; try discriminate;
+        destruct u; try discriminate;
+        destruct v; try discriminate;
+        destruct t2; try discriminate;
+        destruct s; try discriminate;
+        destruct u0; try discriminate;
+        destruct v; try discriminate
+      ].
+  - destruct d; try discriminate.
+    all: try solve [
+      destruct t2; try discriminate;
+      destruct s; try discriminate;
+      destruct u; try discriminate;
+      destruct v; try discriminate
+    ].
+Qed.
+
+Lemma compute_defaultfun__IfThenElse2 : forall t T0 cond t_t,
+  compute_defaultfun t <> Datatypes.Some (Apply (Apply (TyInst (Builtin IfThenElse) T0) cond) t_t).
+Proof.
+  intros.
+  intros Hcon.
+  destruct t.
+  all: inversion Hcon.
+  destruct t1; try discriminate.
+  - destruct t1_1; try discriminate.
+    + destruct t1_1_1; try discriminate.
+      destruct d; try discriminate.
+      destruct t1_1_2; try discriminate.
+      destruct s; try discriminate.
+      destruct u; try discriminate.
+      destruct v; try discriminate.
+      destruct t1_2; try discriminate.
+      destruct s; try discriminate.
+      destruct u0; try discriminate.
+      destruct v; try discriminate.
+      destruct t2; try discriminate.
+      destruct s; try discriminate.
+      destruct u1; try discriminate.
+      destruct v; try discriminate.
+    + destruct d; try discriminate.
+      all: try solve [
+        destruct t1_2; try discriminate;
+        destruct s; try discriminate;
+        destruct u; try discriminate;
+        destruct v; try discriminate;
+        destruct t2; try discriminate;
+        destruct s; try discriminate;
+        destruct u0; try discriminate;
+        destruct v; try discriminate
+      ].
+  - destruct d; try discriminate.
+    all: try solve [
+      destruct t2; try discriminate;
+      destruct s; try discriminate;
+      destruct u; try discriminate;
+      destruct v; try discriminate
+    ].
+Qed.
+
+Lemma eval_builtin_LamAbs : forall v j x T t0,
+    value_builtin v ->
+    ~ v =[j]=> LamAbs x T t0.
+Proof. intros.
+  inversion H; subst.
+  - intros Hcon.
+    inversion Hcon.
+  - intros Hcon.
+    inversion Hcon; subst.
+    all : inversion H4; subst.
+    apply compute_defaultfun__LamAbs in H10.
+    assumption.
+  - intros Hcon.
+    inversion Hcon; subst.
+    + inversion H5; subst.
+      all: inversion H8; subst.
+      apply compute_defaultfun__LamAbs in H15.
+      assumption.
+    + apply compute_defaultfun__LamAbs in H11.
+      assumption.
+    + inversion H5; subst.
+      all: try solve [inversion H6].
+      * inversion H13.
+      * apply compute_defaultfun__IfThenElse2 in H13.
+        assumption.
+      * inversion H11. 
+    + inversion H5; subst.
+      all: try solve [inversion H6].
+      * inversion H13.
+      * apply compute_defaultfun__IfThenElse2 in H13.
+        assumption.
+      * inversion H11.
+Qed.
+
+Lemma eval_builtin_IfThenElse1 : forall v j T cond,
+    value_builtin v ->
+    ~ v =[j]=> Apply (TyInst (Builtin IfThenElse) T) cond.
+Proof.
+  intros.
+  intros Hcon.
+  inversion H; subst.
+  - inversion Hcon.
+  - inversion Hcon; subst.
+    all: try solve [inversion H4].
+    all: try solve [inversion H7].
+    apply compute_defaultfun__IfThenElse1 in H10.
+    assumption.
+  - inversion Hcon; subst.
+    + inversion H5; subst.
+      all: try inversion H8; subst.
+      apply compute_defaultfun__LamAbs in H15.
+      assumption.
+    + inversion H8.
+    + apply compute_defaultfun__IfThenElse1 in H11.
+      assumption.
+    + inversion H8; subst.
+      all: try inversion H5; subst.
+      apply compute_defaultfun__IfThenElse0 in H13.
+      assumption.
+    + inversion H5; subst.
+      all: try inversion H6; subst.
+      * inversion H13.
+      * apply compute_defaultfun__IfThenElse2 in H13.
+        assumption.
+      * inversion H11.
+    + inversion H5; subst.
+      all: try inversion H6.
+      * inversion H13.
+      * apply compute_defaultfun__IfThenElse2 in H13.
+        assumption.
+      * inversion H11.
+Qed.
+
+Lemma eval_builtin_IfThenElse2 : forall v j T cond t_t,
+    value_builtin v ->
+    ~ v =[j]=> Apply (Apply (TyInst (Builtin IfThenElse) T) cond) t_t.
+Proof.
+  intros.
+  intros Hcon.
+  inversion H; subst.
+  - inversion Hcon.
+  - inversion Hcon; subst.
+    all: try solve [inversion H4].
+    all: try solve [inversion H7].
+    * apply compute_defaultfun__IfThenElse2 in H10.
+      assumption.
+    * inversion H8.
+  - inversion Hcon; subst.
+    + inversion H5; subst.
+      all: try inversion H8; subst.
+      apply compute_defaultfun__LamAbs in H15.
+      assumption.
+    + inversion H8.
+    + apply compute_defaultfun__IfThenElse2 in H11.
+      assumption.
+    + inversion H9; subst.
+      all: try inversion H5; subst.
+      * inversion H12.
+      * apply compute_defaultfun__IfThenElse1 in H12.
+        assumption.
+      * inversion H8.
+    + inversion H5; subst.
+      all: try inversion H6; subst.
+      * inversion H13.
+      * apply compute_defaultfun__IfThenElse2 in H13.
+        assumption.
+      * inversion H11.
+    + inversion H5; subst.
+      all: try inversion H6.
+      * inversion H13.
+      * apply compute_defaultfun__IfThenElse2 in H13.
+        assumption.
+      * inversion H11.
+Qed.
+
+
+Lemma eval_IfThenElse2_LamAbs : forall T cond t_t x T0 t0 j,
+    ~ Apply (Apply (TyInst (Builtin IfThenElse) T) cond) t_t =[j]=> LamAbs x T0 t0.
+Proof. Admitted.
+
+
+Definition P_step t t' :=
+  forall j v,
+    t' =[j]=> v ->
+    t =[S j]=> v.
+
+Axiom skip : forall P, P.
+
+Theorem step__eval : forall t t' j v,
+    t --> t' ->
+    t' =[j]=> v ->
+    t =[S j]=> v.
+Proof.
+  intros t t' j v Hstep.
+  generalize dependent v.
+  generalize dependent j.
+  induction Hstep.
+  - (* ST_Let_NilB *) 
+    intros. 
+    destruct recty.
+    + (* recty = NonRec *)
+      apply E_Let.
+      eapply E_NilB_NonRec.
+      assumption.
+    + (* recty = Rec *)
+      apply E_LetRec.
+      eapply E_NilB_Rec.
+      assumption.
+  - (* ST_LetNonRec_ConsB1 *)
+    intros.
+    inversion H. subst.
+    inversion H4. subst. 
+    eapply E_Let.
+    rewrite <- plus_Sn_m.
+    rewrite <- plus_Sn_m.
+    eapply E_ConsB_NonRec.
+    all: eauto.
+  - (* ST_LetNonRec_ConsB2 *)
+    intros.
+    inversion H1. subst.
+    eapply E_Let.
+    replace (S j) with (0 + 1 + j) by reflexivity.
+    eapply E_ConsB_NonRec.
+    all: eauto.
+    eapply eval_value.
+    assumption.
+  - (* ST_Apply1 *)
+    intros.
+    inversion H; subst.
+    + rewrite <- plus_Sn_m.
+      rewrite <- plus_Sn_m.
+      rewrite <- plus_Sn_m.
+      eapply E_Apply.
+      all: eauto.
+    + rewrite <- plus_Sn_m.
+      eapply E_ApplyBuiltin1.
+      all: eauto.
+    + rewrite <- plus_Sn_m.
+      rewrite <- plus_Sn_m.
+      eapply E_ApplyBuiltin2.
+      all: eauto.
+    + rewrite <- plus_Sn_m.
+      eapply E_IfCondition.
+      all: eauto.
+    + eapply E_IfThenBranch.
+      all: eauto.
+    + rewrite <- plus_Sn_m. 
+      eapply E_IfTrue.
+      all: eauto.
+    + rewrite <- plus_Sn_m.
+      eapply E_IfFalse.
+      all: eauto.
+  - (* ST_Apply2 *)
+    intros.
+    inversion H; subst.
+    + inversion H2. subst.
+      rewrite <- plus_Sn_m.
+      rewrite <- plus_Sn_m.
+      rewrite plus_n_Sm.
+      eapply E_Apply.
+      all: eauto.
+    + inversion H2. subst.
+      inversion H3.
+    + inversion H2. subst.
+      inversion H3.
+    + inversion H2.
+    + inversion H4.
+    + inversion H2.
+    + inversion H2.
+  - (* ST_ApplyLamAbs *)
+    intros.
+    replace (S j) with (0 + 0 + 1 + j) by reflexivity.
+    eapply E_Apply.
+    all: eauto.
+    + econstructor.
+    + apply eval_value.
+      assumption.
+  - (* ST_Apply3 *)
+    intros.
+    inversion H0; subst.
+    + apply eval_builtin_LamAbs in H3; auto.
+      destruct H3.
+    + rewrite plus_n_Sm.
+      eapply E_ApplyBuiltin1.
+      all: eauto.
+    + rewrite <- plus_Sn_m.
+      rewrite plus_n_Sm.
+      eapply E_ApplyBuiltin2.
+      all: eauto.
+    + rewrite plus_n_Sm.
+      eapply E_IfCondition.
+      all: eauto.
+    + apply eval_builtin_IfThenElse1 in H5; auto.
+      destruct H5.
+    + apply eval_builtin_IfThenElse2 in H3; auto. 
+      destruct H3.
+    + apply eval_builtin_IfThenElse2 in H3; auto.
+      destruct H3.
+  - (* ST_ApplyBuiltin *)
+    intros.
+    apply compute_defaultfun__to_value in H2 as H4.
+    apply eval_value in H4.
+    unfold P_value in H4.
+    assert (v = v0 /\ j = 0) by (eapply eval__deterministic; eauto).
+    destruct H5. subst.
+    replace 1 with (0 + 0 + 1) by reflexivity.
+    eapply E_ApplyBuiltin2.
+    all: eauto.
+    + apply eval_value.
+      apply V_Builtin.
+      assumption.
+    + apply eval_value.
+      assumption.
+  - (* ST_ApplyIf *)
+    intros.
+    inversion H; subst.
+    + apply eval_IfThenElse2_LamAbs in H2.
+      destruct H2.
+    + apply skip.
+    + apply skip.
+    + apply skip.
+    + apply skip.
+    + apply skip.
+    + apply skip.
+  - (* ST_IfTrue *)
